NuLLReps.thy
@@ -1,5 +1,5 @@
 theory NuLLReps
-  imports NuPrim  "HOL-Library.Word"
+  imports NuPrime  "HOL-Library.Word"
   abbrevs "<own>" = "\<left_fish_tail>"
     and "<none>" = "\<down_fish_tail>"
     and "<object>" = "\<R_arr_tail>"
@@ -8,166 +8,29 @@ begin
 
 text \<open>Semantic data representations\<close>
 
-named_theorems lrep_exps
 declare pair_forall[lrep_exps] pair_exists[lrep_exps]
 
 section \<open>Preliminary notions\<close>
 
-class field = lrep
+class field = lrep \<comment> \<open>a field in the record tuple\<close>
 class field_list = lrep
-
-section \<open>The construction state\<close>
-
-instantiation state :: (lrep) lrep begin
-definition llty_state :: "'a state itself \<Rightarrow> llty" where [simp]: "llty_state _ = la_z"
-instance by standard
-end
-
-section \<open>Owning\<close>
-
-datatype 'a owning = Owning zint 'a (infixr "\<left_fish_tail>" 60) | OwnNone ("\<down_fish_tail>")
-  \<comment> \<open>\<^term>\<open>quantity_of_ownership \<left_fish_tail> data\<close>\<close>
-  
-lemma owning_forall[lrep_exps]: "All P \<longleftrightarrow> P \<down_fish_tail> \<and> (\<forall>z x. P (z \<left_fish_tail> x))" by (metis owning.exhaust) 
-lemma owning_exists[lrep_exps]: "Ex P \<longleftrightarrow> P \<down_fish_tail> \<or> (\<exists>z x. P (z \<left_fish_tail> x))" by (metis owning.exhaust) 
-
-definition "rel1_owning R x y = (case x of zx \<left_fish_tail> ax \<Rightarrow> (case y of zy \<left_fish_tail> ay \<Rightarrow> R ax ay | _ \<Rightarrow> False)  | _ \<Rightarrow> False)"
-lemma [simp]: "rel1_owning R (zx \<left_fish_tail> ax) (zy \<left_fish_tail> ay) = R ax ay"
-  and [simp]: "rel1_owning R \<down_fish_tail> y = False" and [simp]: "rel1_owning R x \<down_fish_tail> = False"
-  unfolding rel1_owning_def by (auto split: owning.split)
-
-subsection \<open>Instantiations\<close>
-
-instantiation owning :: (disposable) disposable begin
-definition disposable_owning :: " 'a owning \<Rightarrow> bool"
-  where "disposable_owning x = (case x of Owning z a \<Rightarrow> disposable a | _ \<Rightarrow> True)"
-lemma [simp]: "disposable (Owning z a) = disposable a" and [simp]: "disposable OwnNone = True"
-  unfolding disposable_owning_def by simp+
-instance by standard
-end
-
-instantiation owning :: (disposable) lrep begin
-definition llty_owning :: " 'a owning itself \<Rightarrow> llty" where "llty_owning _ = la_z"
-instance by standard
-end
-
-instantiation owning :: (disposable) field begin instance by standard end
-instantiation owning :: (disposable) field_list begin instance by standard end
-
-instantiation owning :: (sharing_identical) sharing_identical begin
-definition sharing_identical_owning :: " 'a owning \<Rightarrow> 'a owning \<Rightarrow> bool "
-  where "sharing_identical_owning = rel_owning sharing_identical"
-lemma [simp]: "sharing_identical (Owning z1 x1) (Owning z2 x2) \<longleftrightarrow> (z1 = z2) \<and> sharing_identical x1 x2"
-  and [simp]: "sharing_identical (Owning z1 x1) OwnNone \<longleftrightarrow> False"
-  and [simp]: "sharing_identical OwnNone (Owning z2 x2) \<longleftrightarrow> False"
-  and [simp]: "sharing_identical OwnNone OwnNone \<longleftrightarrow> True"
-  unfolding sharing_identical_owning_def by simp+
-instance proof
-  fix x y z :: \<open>'a owning\<close> and a b :: zint
-  show "sharing_identical x x" by (cases x) simp+
-  show "sharing_identical x y = sharing_identical y x" by (cases x; cases y) auto
-  show "sharing_identical x y \<Longrightarrow> sharing_identical y z \<Longrightarrow> sharing_identical x z" by (cases x; cases y; cases z) (auto intro: sharing_identical_trans)
-qed
-end
-
-instantiation owning :: (type) ownership begin
-definition ownership_owning :: " 'a owning \<Rightarrow> ownership"
-  where "ownership_owning x = (case x of Owning z _ \<Rightarrow> OWS_1 z | OwnNone \<Rightarrow> OWS_0)"
-lemma [simp]: "ownership (Owning z x) = OWS_1 z" and [simp]: "ownership OwnNone = OWS_0"
-  unfolding ownership_owning_def by simp+
-instance by standard
-end
-
-instantiation owning :: (type) share begin
-definition shareable_owning :: " 'a owning \<Rightarrow> bool " where [simp]: "shareable_owning _ = True"
-definition share_owning :: " zint \<Rightarrow> 'a owning \<Rightarrow> 'a owning "
-  where "share_owning z x = (case x of Owning z' a \<Rightarrow> Owning (z' + z) a | _ \<Rightarrow> OwnNone)"
-definition dpriv_owning :: " 'a owning \<Rightarrow> 'a owning" where [simp]: "dpriv_owning x = OwnNone"
-
-lemma [simp]: "share z (Owning z' a) = Owning (z' + z) a" and [simp]: "share z OwnNone = OwnNone"
-  unfolding share_owning_def by simp+
-
-instance proof
-  fix x y z :: \<open>'a owning\<close> and a b :: zint
-  show "share (Gi 0) x = x" by (cases x) auto
-  show "share b (share a x) = share (a + b) x" by (cases x) (auto simp add: add.assoc)
-qed
-end
-
-instantiation owning :: (type) ceq begin
-definition ceqable_owning :: " 'a owning \<Rightarrow> 'a owning \<Rightarrow> bool" where [simp]: "ceqable_owning _ _ = True"
-definition ceq_owning :: " 'a owning \<Rightarrow> 'a owning \<Rightarrow> bool" where [simp]: "ceq_owning _ _ = True"
-instance by standard auto
-end
-
-instantiation owning :: (type) zero begin
-definition zero_owning :: " 'a owning" where [simp]: "zero_owning = \<down_fish_tail>"
-instance by standard
-end
-
-section \<open>Identifier\<close>
-
-datatype identifier = idhypen identifier int (infixl "\<hyphen>" 64) | ID_MEM | ID_CONST string
-  \<comment> \<open>A tree-like structure allowing infinite sub identifier space, like folders where infinite sub-folders can be allocated\<close>
-
-definition alloc_identifier :: "identifier \<Rightarrow> identifier"
-  where "alloc_identifier x = (case x of i\<hyphen>j \<Rightarrow> i\<hyphen>(j + 1))"
-definition alloc_identifier_space :: "identifier \<Rightarrow> identifier"
-  where [simp]: "alloc_identifier_space x = x\<hyphen>0"
-
-lemma [simp]: "alloc_identifier (i\<hyphen>j) = (i\<hyphen>(j + 1))" unfolding alloc_identifier_def by simp
-
-text \<open>Identifier itself is the low representation of identifier source, an abstract value used for assigning identifiers.\<close>
-
-subsection \<open>Instantiations\<close>
-
-instantiation identifier :: lrep begin
-definition llty_identifier :: " identifier itself \<Rightarrow> llty" where [simp]: "llty_identifier _ = la_z"
-definition disposable_identifier :: " identifier \<Rightarrow> bool" where [simp]: "disposable_identifier _ = True"
-instance by standard
-end
-
-instantiation identifier :: field begin instance by standard end
-instantiation identifier :: field_list begin instance by standard end
-
-instantiation identifier :: ceq begin
-definition ceqable_identifier :: "identifier \<Rightarrow> identifier \<Rightarrow> bool" where [simp]: "ceqable_identifier _ _ = True"
-definition ceq_identifier :: "identifier \<Rightarrow> identifier \<Rightarrow> bool" where [simp]: "ceq_identifier _ _ = True"
-instance by standard auto
-end
-
-instantiation identifier :: ownership begin
-definition ownership_identifier :: "identifier \<Rightarrow> ownership" where [simp]: "ownership_identifier _ = OWS_0"
-instance by standard
-end
-
-lemma [\<nu>intro]: "\<nu>Ownership N (\<lambda>x. OWS_0)" for N :: "(identifier, identifier) nu" unfolding \<nu>Ownership_def by simp
-lemma [\<nu>intro]: "\<nu>Disposable S" for S :: "identifier set" unfolding \<nu>Disposable_def by simp
-
-subsection \<open>\<nu>-abstraction for Identifier Source\<close>
-
-definition IdSrc :: "(identifier, identifier) nu" where "IdSrc p x = (p = x)"
-lemma [simp]: "p \<nuLinkL> IdSrc \<nuLinkR> x \<longleftrightarrow> (p = x)" unfolding Refining_ex IdSrc_def by simp
-
-lemma [\<nu>intro]: "\<nu>CEqual IdSrc (\<lambda>x y. True) (\<lambda>x y. True)" unfolding \<nu>CEqual_def by simp
 
 section \<open>Memory address\<close>
 
-datatype memadr = memadr (segment_of_adr: identifier) (offset_of_adr: int) (infix "|+" 60) \<comment> \<open>identifier to the segment, offset in the segment\<close>
-datatype ('spc::len0) memptr = memptr "memadr owning"  \<comment> \<open>'spc : address space\<close>
+datatype ('spc::len0) memptr = memptr memaddr  \<comment> \<open>'spc : address space\<close>
 
-consts size_of :: "llty \<Rightarrow> nat" \<comment> \<open>in unit of bytes\<close>
-consts segment_len :: "identifier \<Rightarrow> nat" \<comment> \<open>in unit of the number of elements\<close>
-consts segment_llty :: "identifier \<Rightarrow> llty" \<comment> \<open>type of the element in the segment\<close>
-consts segment_space :: "identifier \<Rightarrow> nat" \<comment> \<open>LLVM address space of the segment\<close>
+(* consts segment_len :: "identifier \<Rightarrow> nat" \<comment> \<open>in unit of the number of elements\<close> *)
+consts segment_llty :: "msegment \<Rightarrow> llty" \<comment> \<open>type of the element in the segment\<close>
+abbreviation "memaddr_llty adr \<equiv> segment_llty (segment_of_addr adr)"
+consts segment_space :: "memaddr \<Rightarrow> nat" \<comment> \<open>LLVM address space of the segment\<close>
 consts adrspace_capacity :: "nat \<Rightarrow> nat" \<comment> \<open>in unit of bits\<close>
 specification (adrspace_capacity) adrspace_capacity_L0[intro]: "0 < adrspace_capacity spc" by auto
-specification (segment_len) segment_len_max: "segment_len seg < (2::nat) ^ adrspace_capacity (segment_space seg)"
-  proof show "\<forall>seg. (\<lambda>x. 0) seg < (2::nat) ^ adrspace_capacity (segment_space seg)" by auto qed
+(* specification (segment_len) segment_len_max: "segment_len seg < (2::nat) ^ adrspace_capacity (segment_space seg)"
+  proof show "\<forall>seg. (\<lambda>x. 0) seg < (2::nat) ^ adrspace_capacity (segment_space seg)" by auto qed *)
 (* specification (segment_len) segment_len_max: "segment_len seg * size_of (segment_llty seg) < adrspace_capacity (segment_space seg)"
   proof show "\<forall>seg. (\<lambda>x. 0) seg * size_of (segment_llty seg) < adrspace_capacity (segment_space seg)" by auto qed *)
 
-typedef ('b::len0) size_t = "UNIV :: nat set" ..
+(* typedef ('b::len0) size_t = "UNIV :: nat set" ..
 instantiation size_t :: (len0) len begin
 definition len_of_size_t :: "'a size_t itself \<Rightarrow> nat" where [simp]: "len_of_size_t _ = 1 + adrspace_capacity LENGTH('a)"
   \<comment> \<open>it is plus 1 to enable the representation of `negative` offset of the address exorcising any ambiguity.
@@ -175,261 +38,148 @@ definition len_of_size_t :: "'a size_t itself \<Rightarrow> nat" where [simp]: "
     actual total capacity of the address space, 2^31 bytes in the 32 bits machine, so that the size_t in this case still equals
     to that in the actual physical machine. \<close>
 instance by standard auto
-end
+end *)
 
-abbreviation "memadr_len a \<equiv> segment_len (segment_of_adr a)"
-abbreviation "memadr_llty a \<equiv> segment_llty (segment_of_adr a)"
-
-abbreviation within_seg :: "nat \<Rightarrow> memadr \<Rightarrow> bool" where "within_seg len a \<equiv> 0 \<le> offset_of_adr a \<and> nat (offset_of_adr a) + len \<le> memadr_len a"
-
-text \<open>A memory address is represented by an identifier, which is a number sequence, in the specific form
-  \<^term>\<open>id_to_segment\<hyphen>index_of_the_addressing_element_in_this_segment\<close>.
-  
-  The ownership here ensures when releasing the segment to which the address points, which requires the total ownership,
-  all holdings of this address are eliminated, so that no any copy will attend further computation.
-  It is significant when the released segment is recycled and allocated in the future, conflicting with obsolete dangling pointers.
-
-  The address \<^term>\<open>Seg\<hyphen>i\<close> is within the allocated segment only if i < segment_len (Seg\<hyphen>i).
-  Only within addresses can be compared between different segments. In the same segment, only within addresses and that at
-  the end edge can be compared (equality and quantitative).
-
-  Pointer to field of a record structure is not supported, whereas shifting of pointers to elements of an array is supported.
-  Considering field-pointing is an obsolete feature in modern languages, it is worthy to be sacrificed for the sake of the 
-  simplicity of the model, especially when this feature can be replaced by splitting the record into multiple small allocation units
-  at the cost of memory consumption. I admit it leads to memory fragment. This research totally is an adventure.
-  
-  This also means the fix-sized array embedded in the record structure also has to be allocated separately,
-  in a fashion with no distinction with indeterminate-sized array. I admit this hinders both time and memory performance.
-\<close>
-
-lemma memptr_exisits[lrep_exps]: "Ex P \<longleftrightarrow> (\<exists>id. P (memptr id))" by (metis memptr.exhaust) 
-lemma memptr_forall[lrep_exps]: "All P \<longleftrightarrow> (\<forall>id. P (memptr id))" by (metis memptr.exhaust) 
-lemma memadr_exists[lrep_exps]: "Ex P \<longleftrightarrow> (\<exists>s i. P (s |+ i))" by (metis memadr.exhaust)
-lemma memadr_forall[lrep_exps]: "All P \<longleftrightarrow> (\<forall>s i. P (s |+ i))" by (metis memadr.exhaust)
+lemma memptr_exisits[lrep_exps]: "Ex P \<longleftrightarrow> (\<exists>addr. P (memptr addr))" by (metis memptr.exhaust) 
+lemma memptr_forall[lrep_exps]: "All P \<longleftrightarrow> (\<forall>addr. P (memptr addr))" by (metis memptr.exhaust) 
 
 subsection \<open>Instantiations for memptr\<close>
 
 instantiation memptr :: (len0) lrep begin
-definition disposable_memptr :: "'a memptr \<Rightarrow> bool" where [simp]: "disposable_memptr _ = True"
-definition llty_memptr :: "'a memptr itself \<Rightarrow> llty" where [simp]: "llty_memptr _ = la_p LENGTH('a)"
-instance by standard
+definition llty_memptr :: " 'a memptr itself \<Rightarrow> llty" where "llty_memptr _ = llty_pointer LENGTH('a)"
+definition deepize_memptr :: " 'a memptr \<Rightarrow> deep_model"
+  where "deepize_memptr ptr = DM_pointer LENGTH('a) (case_memptr id ptr)"
+definition shallowize_memptr :: " deep_model \<Rightarrow> 'a memptr "
+  where "shallowize_memptr dm = (case dm of DM_pointer _ addr \<Rightarrow> memptr addr)"
+instance apply standard using shallowize_memptr_def deepize_memptr_def by (auto split: memptr.split)
 end
 
 instantiation memptr :: (len0) field begin instance by standard end
 instantiation memptr :: (len0) field_list begin instance by standard end
 
-instantiation memptr :: (len0) sharing_identical begin
-definition sharing_identical_memptr :: " 'a memptr \<Rightarrow> 'a memptr \<Rightarrow> bool" where [simp]: "sharing_identical_memptr = (=)"
+instantiation memptr :: (len0) zero begin
+definition zero_memptr :: "'a memptr" where [simp]: "zero_memptr = memptr 0"
+instance by standard
+end
+
+abbreviation "addr_allocated heap addr \<equiv> Dispose (MemAddress addr) \<in> dom heap"
+
+instantiation memaddr :: ceq begin
+definition ceqable_memaddr :: " heap \<Rightarrow> memaddr \<Rightarrow> memaddr \<Rightarrow> bool"
+  where [simp]: "ceqable_memaddr heap x y = (addr_allocated heap x \<and> addr_allocated heap y)"
+definition ceq_memaddr :: " memaddr \<Rightarrow> memaddr \<Rightarrow> bool" where [simp]: "ceq_memaddr = (=)"
 instance by standard auto
 end
 
-instantiation memptr :: (len0) share begin
-definition shareable_memptr :: " 'a memptr \<Rightarrow> bool" where [simp]: "shareable_memptr _ = True"
-definition share_memptr :: "zint \<Rightarrow> 'a memptr \<Rightarrow> 'a memptr"
-  where "share_memptr z x = (case x of memptr a \<Rightarrow> memptr (share z a))"
-definition dpriv_memptr :: "'a memptr \<Rightarrow> 'a memptr"
-  where "dpriv_memptr x = (case x of memptr a \<Rightarrow> memptr (dpriv a))"
-lemma [simp]: "share z (memptr x) = memptr (share z x)" unfolding share_memptr_def by simp
-lemma [simp]: "dpriv (memptr x) = memptr (dpriv x)" unfolding dpriv_memptr_def by simp
-instance proof
-  fix x :: "'a memptr" and a b :: zint
-  show "share (Gi 0) x = x" by (cases x) simp
-  show "share b (share a x) = share (a + b) x" by (cases x) simp
-qed
-end
-
-instantiation memptr :: (len0) ownership begin
-definition ownership_memptr :: " 'a memptr \<Rightarrow> ownership" where [simp]: "ownership_memptr = case_memptr ownership"
-instance by standard
-end
-
-text \<open>At end of every segment, one additional byte is appended to be allocated more, used for
-  the placeholder of the end pointer, to prevent the potential conflict of addresses between this end
-  and beginning of another segment. One byte is enough, because field-pointing (GetElementPtr) is not
-  supported. Thanking to this, the ceq of the address model can be defined as:\<close>
-
-inductive ceqable_adr where
-  [intro,simp]: "(within_seg 0 a1 \<and> within_seg 0 a2) \<Longrightarrow> ceqable_adr a1 a2"
-| [simp]: "ceqable_adr x y \<Longrightarrow> ceqable_adr y x"
-
 instantiation memptr :: (len0) ceq begin
-definition ceqable_memptr :: " 'a memptr \<Rightarrow> 'a memptr \<Rightarrow> bool" where
-  "ceqable_memptr x y = (case x of memptr a \<Rightarrow> case y of memptr b \<Rightarrow> rel1_owning ceqable_adr a b)"
-lemma [simp]: "ceqable (memptr a) (memptr b) = rel1_owning ceqable_adr a b" unfolding ceqable_memptr_def by simp
+definition ceqable_memptr :: " heap \<Rightarrow> 'a memptr \<Rightarrow> 'a memptr \<Rightarrow> bool" where
+  "ceqable_memptr heap x y = (case x of memptr a \<Rightarrow> case y of memptr b \<Rightarrow>
+    addr_allocated heap a \<and> addr_allocated heap b)"
+lemma [simp]: "ceqable heap (memptr a) (memptr b) = ceqable heap a b" unfolding ceqable_memptr_def by simp
 definition ceq_memptr :: " 'a memptr \<Rightarrow> 'a memptr \<Rightarrow> bool" where [simp]: "ceq_memptr = (=)"
 instance proof
-  fix x y z :: " 'a memptr"
-  show "ceqable x y = ceqable y x" apply (cases x; cases y) apply simp subgoal for a b by (cases a; cases b) auto done
-  show "ceqable x x \<Longrightarrow> ceq x x" and "ceqable x y \<Longrightarrow> ceq x y = ceq y x"
-    and "ceqable x y \<Longrightarrow> ceqable y z \<Longrightarrow> ceqable x z \<Longrightarrow> ceq x y \<Longrightarrow> ceq y z \<Longrightarrow> ceq x z" by auto+
+  fix x y z :: " 'a memptr" and h :: heap
+  show "ceqable h x y = ceqable h y x" by (cases x; cases y) simp
+  show "ceqable h x x \<Longrightarrow> ceq x x" and "ceqable h x y \<Longrightarrow> ceq x y = ceq y x"
+    and "ceqable h x y \<Longrightarrow> ceqable h y z \<Longrightarrow> ceqable h x z \<Longrightarrow> ceq x y \<Longrightarrow> ceq y z \<Longrightarrow> ceq x z" by auto+
 qed
 end
-
-instantiation memptr :: (len0) zero begin
-definition zero_memptr :: " 'a memptr" where [simp]: "zero_memptr = memptr \<down_fish_tail>"
-instance by standard
-end
-
-lemma [\<nu>intro]: "\<nu>Disposable S" for S :: "('spc0::len0) memptr set" unfolding \<nu>Disposable_def by simp
 
 subsection \<open>\<nu>-abstraction\<close>
 
-subsubsection \<open>RawPointer\<close>
+subsubsection \<open>None typed Pointer\<close>
 
-definition RawPtr' :: "('spc::len0) itself \<Rightarrow> ('spc memptr, memadr owning) nu"
-  where "RawPtr' _ p x = (case p of (memptr i) \<Rightarrow> i = x)"
-syntax "_RawPtr'_" :: "type \<Rightarrow> logic" (\<open>RawPtr'[_']\<close>)
-translations "RawPtr['x]" == "CONST RawPtr' (TYPE('x))" 
-abbreviation "RawPtr \<equiv> RawPtr[0]"
-
-lemma [simp]: "memptr i \<nuLinkL> RawPtr['spc::len0] \<nuLinkR> i' \<longleftrightarrow> (i = i')" unfolding RawPtr'_def Refining_ex by auto
-lemma [elim,\<nu>elim]: "z \<left_fish_tail> i \<ratio> RawPtr['spc::len0] \<Longrightarrow> C \<Longrightarrow> C" unfolding Inhabited_def by (simp add: lrep_exps)
-
-lemma [\<nu>intro]: "\<nu>Share RawPtr['spc::len0] (\<lambda>x. True) share" unfolding \<nu>Share_def by (simp add: lrep_exps)
-lemma [\<nu>intro]: "\<nu>ShrIdentical RawPtr['spc::len0] (=)" unfolding \<nu>ShrIdentical_def by (simp add: lrep_exps)
-lemma [\<nu>intro]: "\<nu>Deprive RawPtr['spc::len0] dpriv" unfolding \<nu>Deprive_def by (simp add: lrep_exps)
-lemma [\<nu>intro]: "\<nu>Ownership RawPtr['spc::len0] ownership" unfolding \<nu>Ownership_def by (simp add: lrep_exps)
-lemma [\<nu>intro]: "\<nu>Zero RawPtr['spc::len0] \<down_fish_tail>" unfolding \<nu>Zero_def by simp
-
-subsubsection \<open>ComparablePointer\<close>
-
-definition ComparablePtr' :: "('spc::len0) itself \<Rightarrow> ('spc memptr, memadr owning) nu"
-  where "ComparablePtr' _ p x = (case p of (memptr i) \<Rightarrow> (i = x) \<and> pred_owning (within_seg 0) i)"
-syntax "_ComparablePtr'_" :: "type \<Rightarrow> logic" (\<open>ComparablePtr'[_']\<close>)
-translations "ComparablePtr['x]" == "CONST ComparablePtr' (TYPE('x))" 
-abbreviation "ComparablePtr \<equiv> ComparablePtr[0]"
-
-lemma [simp]: "memptr i \<nuLinkL> ComparablePtr['spc::len0] \<nuLinkR> i' \<longleftrightarrow> (i = i') \<and> pred_owning (within_seg 0) i'" unfolding ComparablePtr'_def Refining_ex by auto
-lemma [elim,\<nu>elim]: "z \<left_fish_tail> i \<ratio> ComparablePtr['spc::len0] \<Longrightarrow> (within_seg 0 i \<Longrightarrow> C) \<Longrightarrow> C" unfolding Inhabited_def by (simp add: lrep_exps)
-
-lemma [\<nu>intro]: "\<nu>CEqual ComparablePtr['spc::len0] (rel1_owning (\<lambda>x y. True)) (=)" unfolding \<nu>CEqual_def by (simp add: lrep_exps)
-lemma [\<nu>intro]: "\<nu>Share ComparablePtr['spc::len0] (\<lambda>x. True) share" unfolding \<nu>Share_def by (simp add: lrep_exps)
-lemma [\<nu>intro]: "\<nu>ShrIdentical ComparablePtr['spc::len0] (=)" unfolding \<nu>ShrIdentical_def by (simp add: lrep_exps)
-lemma [\<nu>intro]: "\<nu>Deprive ComparablePtr['spc::len0] dpriv" unfolding \<nu>Deprive_def by (simp add: lrep_exps)
-lemma [\<nu>intro]: "\<nu>Ownership ComparablePtr['spc::len0] ownership" unfolding \<nu>Ownership_def by (simp add: lrep_exps)
-lemma [\<nu>intro]: "\<nu>Zero ComparablePtr['spc::len0] \<down_fish_tail>" unfolding \<nu>Zero_def by simp
-
-subsubsection \<open>Slide pointer\<close>
-
-definition SlidePtr' :: " ('spc::len0) itself \<Rightarrow> llty \<Rightarrow> ('spc memptr, memadr owning) nu"
-  where "SlidePtr' _ ty p x = (case p of (memptr ap) \<Rightarrow> ap = x \<and> pred_owning (\<lambda>a. memadr_llty a = ty) x)"
-syntax "_SlidePtr'_" :: "type \<Rightarrow> logic" (\<open>SlidePtr'[_']\<close>)
-translations "SlidePtr['x]" == "CONST SlidePtr' (TYPE('x))" 
-abbreviation "SlidePtr \<equiv> SlidePtr[0]"
-
-lemma [simp]: "memptr i \<nuLinkL> SlidePtr['spc::len0] ty \<nuLinkR> i' \<longleftrightarrow> (i = i') \<and> pred_owning (\<lambda>a. memadr_llty a = ty) i'"
-  unfolding SlidePtr'_def Refining_ex by auto
-lemma [elim,\<nu>elim]: " z \<left_fish_tail> a \<ratio> SlidePtr['spc::len0] ty \<Longrightarrow> (memadr_llty a = ty \<Longrightarrow> C) \<Longrightarrow> C" unfolding Inhabited_def by (cases a) (simp add: lrep_exps)
-
-lemma [\<nu>intro]: "\<nu>CEqual (SlidePtr['spc::len0] ty) (rel1_owning ceqable_adr) (=)" unfolding \<nu>CEqual_def by (simp add: lrep_exps)
-lemma [\<nu>intro]: "\<nu>Share (SlidePtr['spc::len0] ty) (\<lambda>x. True) share" unfolding \<nu>Share_def by (simp add: lrep_exps)
-lemma [\<nu>intro]: "\<nu>ShrIdentical (SlidePtr['spc::len0] ty) (=)" unfolding \<nu>ShrIdentical_def by (simp add: lrep_exps)
-lemma [\<nu>intro]: "\<nu>Deprive (SlidePtr['spc::len0] ty) dpriv" unfolding \<nu>Deprive_def by (simp add: lrep_exps)
-lemma [\<nu>intro]: "\<nu>Ownership (SlidePtr['spc::len0] ty) ownership" unfolding \<nu>Ownership_def by (simp add: lrep_exps)
-lemma [\<nu>intro]: "\<nu>Zero (SlidePtr['spc::len0] ty) \<down_fish_tail>" unfolding \<nu>Zero_def by simp
-
-subsubsection \<open>Typed Pointer\<close>
-
-definition Pointer' :: "('spc::len0) itself \<Rightarrow> llty \<Rightarrow> ('spc memptr, memadr owning) nu"
-  where "Pointer' _ ty p x = (case p of (memptr i) \<Rightarrow> (i = x) \<and> pred_owning (within_seg 0) x \<and> pred_owning (\<lambda>a. memadr_llty a = ty) x)"
+definition Pointer' :: "('spc::len0) itself \<Rightarrow> ('spc memptr, memaddr) \<nu>"
+  where "Pointer' _ h p x = (case p of (memptr i) \<Rightarrow> (i = x))"
 syntax "_Pointer'_" :: "type \<Rightarrow> logic" (\<open>Pointer'[_']\<close>)
 translations "Pointer['x]" == "CONST Pointer' (TYPE('x))" 
 abbreviation "Pointer \<equiv> Pointer[0]"
 
-lemma [simp]: "memptr i \<nuLinkL> Pointer['spc::len0] ty \<nuLinkR> i' \<longleftrightarrow>
-    (i = i') \<and> pred_owning (within_seg 0) i \<and> pred_owning (\<lambda>a. memadr_llty a = ty) i'"
-  unfolding Pointer'_def Refining_ex by auto
-lemma [elim,\<nu>elim]: " z \<left_fish_tail> a \<ratio> Pointer['spc::len0] ty \<Longrightarrow> (memadr_llty a = ty \<Longrightarrow> C) \<Longrightarrow> C" unfolding Inhabited_def by (cases a) (simp add: lrep_exps)
+lemma [simp]: "[heap] memptr i \<nuLinkL> Pointer' spc \<nuLinkR> i' \<longleftrightarrow> (i = i')" unfolding Pointer'_def Refining_ex by auto
+lemma [elim,\<nu>elim]: " addr \<ratio> (Pointer' spc) \<Longrightarrow> C \<Longrightarrow> C" unfolding Inhabited_def by (simp add: lrep_exps)
+lemma [\<nu>intro]: "\<nu>Equal (Pointer' spc) ceqable (=)" unfolding \<nu>Equal_def by (simp add: lrep_exps)
+lemma [\<nu>intro]: "\<nu>Zero (Pointer' spc) 0" unfolding \<nu>Zero_def by simp
+lemma [\<nu>intro]: "\<nu>Resources (Pointer' spc) (\<lambda>x. {})" unfolding \<nu>def by (simp add: lrep_exps)
 
-lemma [\<nu>intro]: "\<nu>CEqual (Pointer['spc::len0] ty) (rel1_owning ceqable_adr) (=)" unfolding \<nu>CEqual_def by (simp add: lrep_exps)
-lemma [\<nu>intro]: "\<nu>Share (Pointer['spc::len0] ty) (\<lambda>x. True) share" unfolding \<nu>Share_def by (simp add: lrep_exps)
-lemma [\<nu>intro]: "\<nu>ShrIdentical (Pointer['spc::len0] ty) (=)" unfolding \<nu>ShrIdentical_def by (simp add: lrep_exps)
-lemma [\<nu>intro]: "\<nu>Deprive (Pointer['spc::len0] ty) dpriv" unfolding \<nu>Deprive_def by (simp add: lrep_exps)
-lemma [\<nu>intro]: "\<nu>Ownership (Pointer['spc::len0] ty) ownership" unfolding \<nu>Ownership_def by (simp add: lrep_exps)
-lemma [\<nu>intro]: "\<nu>Zero (Pointer['spc::len0] ty) \<down_fish_tail>" unfolding \<nu>Zero_def by simp
+subsubsection \<open>Typed Pointer\<close>
+
+definition TypedPtr' :: "('spc::len0) itself \<Rightarrow> llty \<Rightarrow> ('spc memptr, memaddr) \<nu>"
+  where "TypedPtr' _ ty h p x = (case p of (memptr i) \<Rightarrow> (i = x) \<and> memaddr_llty i = ty)"
+syntax "_TypedPtr'_" :: "type \<Rightarrow> logic" (\<open>TypedPtr'[_']\<close>)
+translations "TypedPtr['x]" == "CONST TypedPtr' (TYPE('x))" 
+abbreviation "TypedPtr \<equiv> TypedPtr[0]"
+
+lemma [simp]: "[heap] memptr i \<nuLinkL> TypedPtr' spc ty \<nuLinkR> i' \<longleftrightarrow> (i = i') \<and> memaddr_llty i = ty"
+  unfolding TypedPtr'_def Refining_ex by auto
+lemma [elim,\<nu>elim]: " addr \<ratio> TypedPtr' spc ty \<Longrightarrow> (memaddr_llty addr = ty \<Longrightarrow> C) \<Longrightarrow> C"
+  unfolding Inhabited_def by (simp add: lrep_exps)
+lemma [\<nu>intro]: "\<nu>Equal (TypedPtr' spc ty) ceqable (=)" unfolding \<nu>Equal_def by (simp add: lrep_exps)
+lemma [\<nu>intro]: "\<nu>Resources (TypedPtr' spc ty) (\<lambda>x. {})" unfolding \<nu>def by (simp add: lrep_exps)
 
 subsubsection \<open>Casts\<close>
 
-named_theorems slide_\<nu>cast and fixtyp_\<nu>cast and freetyp_\<nu>cast
-
-lemma [\<nu>intro, slide_\<nu>cast]:
-  "\<^bold>c\<^bold>a\<^bold>s\<^bold>t a \<tycolon> Pointer['spc] ty \<longmapsto> a \<tycolon> SlidePtr['spc::len0] ty \<^bold>m\<^bold>e\<^bold>a\<^bold>n\<^bold>w\<^bold>h\<^bold>i\<^bold>l\<^bold>e pred_owning (within_seg 0) a "
-  unfolding Cast_def by (cases a) (auto split: memadr.split simp add: lrep_exps)
-
-lemma [\<nu>intro, slide_\<nu>cast]:
-  "\<^bold>p\<^bold>r\<^bold>e\<^bold>m\<^bold>i\<^bold>s\<^bold>e pred_owning (\<lambda>x. memadr_llty x = ty) a \<Longrightarrow>
-    \<^bold>c\<^bold>a\<^bold>s\<^bold>t a \<tycolon> FreePtr['spc] \<longmapsto> a \<tycolon> SlidePtr['spc::len0] ty \<^bold>m\<^bold>e\<^bold>a\<^bold>n\<^bold>w\<^bold>h\<^bold>i\<^bold>l\<^bold>e pred_owning (within_seg 0) a "
-  unfolding Cast_def by (cases a) (auto split: memadr.split simp add: lrep_exps)
+named_theorems fixtyp_\<nu>cast and freetyp_\<nu>cast
 
 lemma [\<nu>intro, fixtyp_\<nu>cast]:
-  "\<^bold>p\<^bold>r\<^bold>e\<^bold>m\<^bold>i\<^bold>s\<^bold>e pred_owning (within_seg 0) a \<Longrightarrow>
-    \<^bold>c\<^bold>a\<^bold>s\<^bold>t a \<tycolon> SlidePtr['spc] ty \<longmapsto> a \<tycolon> Pointer['spc::len0] ty"
-  unfolding Cast_def by (cases a) (auto simp add: lrep_exps split: memadr.split)
-
-lemma [\<nu>intro, fixtyp_\<nu>cast]:
-  "\<^bold>p\<^bold>r\<^bold>e\<^bold>m\<^bold>i\<^bold>s\<^bold>e pred_owning (\<lambda>x. memadr_llty x = ty) a \<Longrightarrow>
-    \<^bold>c\<^bold>a\<^bold>s\<^bold>t a \<tycolon> FreePtr['spc] \<longmapsto> a \<tycolon> Pointer['spc::len0] ty"
-  unfolding Cast_def by (cases a) (auto simp add: lrep_exps split: memadr.split)
+  "\<^bold>p\<^bold>r\<^bold>e\<^bold>m\<^bold>i\<^bold>s\<^bold>e memaddr_llty addr = ty \<Longrightarrow>
+    \<^bold>c\<^bold>a\<^bold>s\<^bold>t addr \<tycolon> Pointer['spc] \<longmapsto> addr \<tycolon> TypedPtr['spc::len0] ty"
+  unfolding Cast_def by (cases addr) (auto simp add: lrep_exps split: memaddr.split)
 
 lemma [\<nu>intro, freetyp_\<nu>cast]:
-  "\<^bold>p\<^bold>r\<^bold>e\<^bold>m\<^bold>i\<^bold>s\<^bold>e pred_owning (within_seg 0) a \<Longrightarrow>
-    \<^bold>c\<^bold>a\<^bold>s\<^bold>t a \<tycolon> SlidePtr['spc] ty \<longmapsto> a \<tycolon> FreePtr['spc::len0]  \<^bold>m\<^bold>e\<^bold>a\<^bold>n\<^bold>w\<^bold>h\<^bold>i\<^bold>l\<^bold>e pred_owning (\<lambda>x. memadr_llty x = ty) a"
-  unfolding Cast_def by (cases a) (auto simp add: lrep_exps split: memadr.split)
-
-lemma [\<nu>intro, freetyp_\<nu>cast]:
-  "\<^bold>c\<^bold>a\<^bold>s\<^bold>t a \<tycolon> Pointer['spc] ty \<longmapsto> a \<tycolon> FreePtr['spc::len0] \<^bold>m\<^bold>e\<^bold>a\<^bold>n\<^bold>w\<^bold>h\<^bold>i\<^bold>l\<^bold>e pred_owning (\<lambda>x. memadr_llty x = ty) a"
-  unfolding Cast_def by (cases a) (auto simp add: lrep_exps split: memadr.split)
+  "\<^bold>c\<^bold>a\<^bold>s\<^bold>t addr \<tycolon> TypedPtr['spc] ty \<longmapsto> addr \<tycolon> Pointer['spc::len0] \<^bold>m\<^bold>e\<^bold>a\<^bold>n\<^bold>w\<^bold>h\<^bold>i\<^bold>l\<^bold>e memaddr_llty addr = ty"
+  unfolding Cast_def by (cases addr) (auto simp add: lrep_exps split: memaddr.split)
 
 section \<open>Void\<close>
 
-instantiation void :: naive_lrep begin
-definition share_void :: "zint \<Rightarrow> void \<Rightarrow> void" where [simp]: "share_void z = id"
-definition shareable_void :: "void \<Rightarrow> bool" where [simp]: "shareable_void _ = True"
-definition sharing_identical_void :: "void \<Rightarrow> void \<Rightarrow> bool" where [simp]: "sharing_identical_void x y = True"
-definition dpriv_void :: "void \<Rightarrow> void" where [simp]: "dpriv_void x = x"
-instance by standard auto
+datatype void = void
+declare void.split[split]
+
+lemma [simp]: "x = y" for x :: void by (cases x; cases y) fast
+
+subsection \<open>Settings\<close>
+
+instantiation void :: stack begin
+definition llty_void :: "void itself \<Rightarrow> llty" where "llty_void _ = llty_nil"
+definition deepize_void :: "void \<Rightarrow> deep_model" where "deepize_void _ = DM_none"
+instance by standard auto 
 end
+
 
 instantiation void :: field begin instance by standard end
 instantiation void :: field_list begin instance by standard end
-
-instantiation void :: ownership begin
-definition ownership_void :: "void \<Rightarrow> ownership" where [simp]: "ownership_void _ = OWS_0"
-instance by standard
-end
 
 instantiation void :: zero begin
 definition zero_void :: "void" where [simp]: "zero_void = void"
 instance by standard
 end
 
-lemma [\<nu>intro]: "\<nu>Ownership N (\<lambda>x. OWS_0)" for N :: "(void, 'b) nu" unfolding \<nu>Ownership_def by simp
+
+subsection \<open>Abstractor\<close>
+
+definition Void :: "heap \<Rightarrow> void set" where "Void _ = {void}" 
+text \<open>The name `void` coincides that, when a procedure has no input arguments,
+  the \<nu>-type for the input would exactly be @{term Void}. \<close>
+lemma [simp,intro]: "void \<in> Void res" unfolding Void_def by simp
+lemma [simp,intro]: "Inhabited Void" unfolding Inhabited_def by auto
+lemma [elim!, \<nu>elim]: "Inhabited Void \<Longrightarrow> C \<Longrightarrow> C" .
+lemma [intro]: "NuSet Void" unfolding NuSet_def Void_def by simp
+lemma [intro]: "\<nu>Resources_of_set Void {}" unfolding \<nu>Resources_of_set_def Void_def by fast
+(*translations "a" <= "a \<^bold>a\<^bold>n\<^bold>d CONST Void"*)
 
 section \<open>The integer data type\<close>
 
 subsection \<open>Lrep instantiations\<close>
 
-instantiation word :: (len) naive_lrep
-begin
-definition llty_word :: "'a word itself \<Rightarrow> llty" where [simp]: "llty_word _ = la_i LENGTH('a)"
-definition share_word :: "zint \<Rightarrow> 'a word \<Rightarrow> 'a word" where [simp]: "share_word z = id"
-definition shareable_word :: "'a word \<Rightarrow> bool" where [simp]: "shareable_word _ = True"
-definition sharing_identical_word :: "'a word \<Rightarrow> 'a word \<Rightarrow> bool" where [simp]: "sharing_identical_word x y = True"
-definition dpriv_word :: "'a word \<Rightarrow> 'a word" where [simp]: "dpriv_word x = x"
-definition disposable_word :: "'a word \<Rightarrow> bool" where [simp]: "disposable_word _ = True"
-instance by standard auto
+instantiation word :: (len) lrep begin
+definition llty_word :: "'a word itself \<Rightarrow> llty" where [simp]: "llty_word _ = llty_int LENGTH('a)"
+definition deepize_word :: " 'a word \<Rightarrow> deep_model " where "deepize_word x = DM_int LENGTH('a) (unat x)"
+definition shallowize_word :: " deep_model \<Rightarrow> 'a word" where "shallowize_word x = (case x of DM_int _ n \<Rightarrow> of_nat n)"
+instance apply standard using deepize_word_def shallowize_word_def by auto
 end
-
-instantiation word :: (len) ownership begin
-definition ownership_word :: " 'a word \<Rightarrow> ownership" where [simp]: "ownership_word _ = OWS_0"
-instance by standard
-end
-
-lemma [\<nu>intro]: "\<nu>Ownership N (\<lambda>x. OWS_0)" for N :: "(('len::len) word, 'b) nu" unfolding \<nu>Ownership_def by simp
 
 instantiation word :: (len) ceq
 begin
-definition ceqable_word :: "'a word \<Rightarrow> 'a word \<Rightarrow> bool" where [simp]: "ceqable_word x y = True"
+definition ceqable_word :: "heap \<Rightarrow> 'a word \<Rightarrow> 'a word \<Rightarrow> bool" where [simp]: "ceqable_word _ x y = True"
 definition ceq_word :: "'a word \<Rightarrow>  'a word \<Rightarrow> bool" where [simp]: "ceq_word x y = (x = y)"
 instance by standard (auto+)
 end
@@ -441,35 +191,36 @@ subsection \<open>Basic \<nu>-abstractions based on integer type\<close>
 
 subsubsection \<open>Natural number\<close>
 
-definition NuNat :: "('a::len) itself \<Rightarrow> ('a word, nat) nu" where "NuNat _ p x = (unat p = x)"
+definition NuNat :: "('a::len) itself \<Rightarrow> ('a word, nat) \<nu>" where "NuNat _ h p x = (unat p = x)"
 syntax "_NuNat_" :: "type \<Rightarrow> logic" (\<open>\<nat>'[_']\<close>)
 translations "\<nat>['x]" == "CONST NuNat (TYPE('x))" 
 
-lemma [simp]: "p \<nuLinkL> NuNat b \<nuLinkR> x \<equiv> (unat p = x)" unfolding NuNat_def Refining_ex by auto
+lemma [simp]: "[heap] p \<nuLinkL> NuNat b \<nuLinkR> x \<equiv> (unat p = x)" unfolding NuNat_def Refining_ex by auto
 lemma [elim,\<nu>elim]: "x \<ratio> \<nat>['b::len] \<Longrightarrow> (x < 2^LENGTH('b) \<Longrightarrow> C) \<Longrightarrow> C" unfolding Inhabited_def by auto
 
-lemma [\<nu>intro]: "\<nu>CEqual (NuNat b) (\<lambda>x y. True) (=)"
-  unfolding \<nu>CEqual_def by (auto simp add: unsigned_word_eqI)
+lemma [\<nu>intro]: "\<nu>Equal (NuNat b) (\<lambda>heap x y. True) (=)"
+  unfolding \<nu>Equal_def by (auto simp add: unsigned_word_eqI)
 lemma [\<nu>intro]: "\<nu>Zero (NuNat b) 0" unfolding \<nu>Zero_def by simp
+lemma [\<nu>intro]: "\<nu>Resources (NuNat b) (\<lambda>x. {})" unfolding \<nu>def by simp
 
-definition NuNatRound :: "('a::len) itself \<Rightarrow> ('a word, nat) nu" where "NuNatRound _ p x = (p = of_nat x)"
+definition NuNatRound :: "('a::len) itself \<Rightarrow> ('a word, nat) \<nu>" where "NuNatRound _ h p x = (p = of_nat x)"
 syntax "_NuNatRound_" :: "type \<Rightarrow> logic" (\<open>\<nat>\<^sup>r'[_']\<close>)
 translations "\<nat>\<^sup>r['x]" == "CONST NuNatRound (TYPE('x))" 
 
-lemma [simp]: "p \<nuLinkL> NuNatRound b \<nuLinkR> x \<equiv> (p = of_nat x)" unfolding NuNatRound_def Refining_ex by auto
+lemma [simp]: "[heap] p \<nuLinkL> NuNatRound b \<nuLinkR> x \<equiv> (p = of_nat x)" unfolding NuNatRound_def Refining_ex by auto
 lemma [\<nu>intro]: "\<nu>Zero (NuNatRound b) 0" unfolding \<nu>Zero_def by simp
 
 subsubsection \<open>Integer\<close>
 
-definition NuInt :: "('a::len) itself \<Rightarrow> ('a word, int) nu" where "NuInt _ p x = (sint p = x)"
+definition NuInt :: "('a::len) itself \<Rightarrow> ('a word, int) \<nu>" where "NuInt _ h p x = (sint p = x)"
 syntax "_NuInt_" :: "type \<Rightarrow> logic" (\<open>\<int>'[_']\<close>)
 translations "\<int>['x]" == "CONST NuInt (TYPE('x))" 
 
-lemma [simp]: "p \<nuLinkL> NuInt b \<nuLinkR> x \<equiv> (sint p = x)" unfolding NuInt_def Refining_ex by auto
+lemma [simp]: "[heap] p \<nuLinkL> NuInt b \<nuLinkR> x \<equiv> (sint p = x)" unfolding NuInt_def Refining_ex by auto
 lemma [elim,\<nu>elim]: "x \<ratio> \<int>['b::len] \<Longrightarrow> (x < 2^(LENGTH('b) - 1) \<Longrightarrow> -(2^(LENGTH('b)-1)) \<le> x \<Longrightarrow> C) \<Longrightarrow> C"
   unfolding Inhabited_def apply simp by (metis One_nat_def sint_ge sint_lt) 
 
-lemma [\<nu>intro]: "\<nu>CEqual (NuInt b) (\<lambda>x y. True) (=)" unfolding \<nu>CEqual_def by (auto simp add: signed_word_eqI) 
+lemma [\<nu>intro]: "\<nu>Equal (NuInt b) (\<lambda>h x y. True) (=)" unfolding \<nu>Equal_def by (auto simp add: signed_word_eqI) 
 lemma [\<nu>intro]: "\<nu>Zero (NuInt b) 0" unfolding \<nu>Zero_def by simp
 
 subsubsection \<open>Boolean\<close>
@@ -481,9 +232,9 @@ lemma [simp]: "(x \<noteq> 1) = (x = 0)" for x :: "1 word" proof -
   then show ?thesis  by auto
 qed
 
-definition NuBool :: "(1 word, bool) nu" ("\<bool>") where "NuBool p x = ((p = 1) = x)"
-lemma [simp]: "p \<nuLinkL> \<bool> \<nuLinkR> x \<longleftrightarrow> (p = 1) = x" unfolding NuBool_def Refining_ex by simp
-lemma [\<nu>intro]: "\<nu>CEqual \<bool> (\<lambda>x y. True)  (=)" unfolding \<nu>CEqual_def by auto
+definition NuBool :: "(1 word, bool) \<nu>" ("\<bool>") where "NuBool h p x = ((p = 1) = x)"
+lemma [simp]: "[heap] p \<nuLinkL> \<bool> \<nuLinkR> x \<longleftrightarrow> (p = 1) = x" unfolding NuBool_def Refining_ex by simp
+lemma [\<nu>intro]: "\<nu>Equal \<bool> (\<lambda>heap x y. True)  (=)" unfolding \<nu>Equal_def by auto
 
 lemma [\<nu>intro]: "\<nu>Zero NuBool False" unfolding \<nu>Zero_def by simp
 
@@ -497,35 +248,9 @@ instantiation prod :: (zero, zero) zero begin
 definition zero_prod :: "'a \<times> 'b" where [simp]: "zero_prod = (0,0)"
 instance by standard
 end
-
-instantiation prod :: (ownership, ownership) ownership begin
-definition ownership_prod :: " 'a \<times> 'b \<Rightarrow> ownership"
-  where "ownership_prod x = (case x of (a,b) \<Rightarrow> OWS_C (ownership a) (ownership b))"
-lemma [simp]: "ownership (a,b) = OWS_C (ownership a) (ownership b)" unfolding ownership_prod_def by simp
-instance by standard
-end
-
-instantiation prod :: (sharing_identical, sharing_identical) sharing_identical begin
-definition sharing_identical_prod :: "('a \<times> 'b) \<Rightarrow> ('a \<times> 'b) \<Rightarrow> bool" where "sharing_identical_prod = sharing_identical \<times>\<^sub>r sharing_identical"
-lemma [simp]: "sharing_identical (a1,b1) (a2,b2) \<longleftrightarrow> sharing_identical a1 a2 \<and> sharing_identical b1 b2"
-  unfolding sharing_identical_prod_def by simp
-instance by standard (auto intro: sharing_identical_trans)
-end
-
-instantiation prod :: (share, share) share begin
-definition shareable_prod :: "('a \<times> 'b) \<Rightarrow> bool" where "shareable_prod = shareable \<times>\<^sub>p shareable"
-definition share_prod :: "zint \<Rightarrow> 'a \<times> 'b \<Rightarrow> 'a \<times> 'b" where [simp]: "share_prod z x = (case x of (a,b) \<Rightarrow> (share z a, share z b))"
-definition dpriv_prod :: "'a \<times> 'b \<Rightarrow> 'a \<times> 'b" where [simp]: "dpriv_prod x = (case x of (a,b) \<Rightarrow> (dpriv a, dpriv b))"
-lemma [simp]: "shareable (a,b) \<longleftrightarrow> shareable a \<and> shareable b" unfolding shareable_prod_def by simp
-instance by standard auto
-end
-
-instantiation prod :: (naive_lrep, naive_lrep) naive_lrep
-  begin instance by standard auto end
-
 instantiation prod :: (ceq, ceq) ceq begin
-definition ceqable_prod :: "'a \<times> 'b \<Rightarrow> 'a \<times> 'b \<Rightarrow> bool" where "ceqable_prod  = ceqable \<times>\<^sub>r ceqable"
-lemma [simp]: "ceqable (a1,b1) (a2,b2) \<longleftrightarrow> ceqable a1 a2 \<and> ceqable b1 b2" unfolding ceqable_prod_def by auto
+definition ceqable_prod :: "heap \<Rightarrow> 'a \<times> 'b \<Rightarrow> 'a \<times> 'b \<Rightarrow> bool" where "ceqable_prod heap = ceqable heap \<times>\<^sub>r ceqable heap"
+lemma [simp]: "ceqable heap (a1,b1) (a2,b2) \<longleftrightarrow> ceqable heap a1 a2 \<and> ceqable heap b1 b2" unfolding ceqable_prod_def by auto
 definition ceq_prod :: "'a \<times> 'b \<Rightarrow> 'a \<times> 'b \<Rightarrow> bool" where "ceq_prod = ceq \<times>\<^sub>r ceq"
 lemma [simp]: "ceq (a1,b1) (a2,b2) \<longleftrightarrow> ceq a1 a2 \<and> ceq b1 b2" unfolding ceq_prod_def by auto
 instance by standard (auto intro: ceq_trans)
@@ -533,17 +258,13 @@ end
 
 subsection \<open>Fusion \<nu>-abstraction\<close>
 
-definition Fusion :: "('a1::lrep,'b1) nu \<Rightarrow> ('a2::lrep,'b2) nu \<Rightarrow> ('a1 \<times> 'a2, 'b1 \<times> 'b2) nu" (infixr "\<nuFusion>" 70) 
-  where "Fusion N M p x = (case p of (p1,p2) \<Rightarrow> case x of (x1,x2) \<Rightarrow> (p1 \<nuLinkL> N \<nuLinkR> x1) \<and> (p2 \<nuLinkL> M \<nuLinkR> x2))"
+definition Fusion :: "('a1::lrep,'b1) \<nu> \<Rightarrow> ('a2::lrep,'b2) \<nu> \<Rightarrow> ('a1 \<times> 'a2, 'b1 \<times> 'b2) \<nu>" (infixr "\<nuFusion>" 70) 
+  where "Fusion N M heap p x = (case p of (p1,p2) \<Rightarrow> case x of (x1,x2) \<Rightarrow> 
+    ([heap] p1 \<nuLinkL> N \<nuLinkR> x1) \<and> ([heap] p2 \<nuLinkL> M \<nuLinkR> x2))"
 
-lemma [simp]: "(p1,p2) \<nuLinkL> N \<nuFusion> M \<nuLinkR> (x1,x2) \<longleftrightarrow> (p1 \<nuLinkL> N \<nuLinkR> x1) \<and> (p2 \<nuLinkL> M \<nuLinkR> x2)" unfolding Fusion_def Refining_ex by simp
-lemma [elim,\<nu>elim]: "(x1,x2) \<ratio> N1 \<nuFusion> N2 \<Longrightarrow> (x1 \<ratio> N1 \<Longrightarrow> x2 \<ratio> N2 \<Longrightarrow> C) \<Longrightarrow> C" unfolding Inhabited_def by simp
+lemma [simp]: "[heap] (p1,p2) \<nuLinkL> N \<nuFusion> M \<nuLinkR> (x1,x2) \<longleftrightarrow> ([heap] p1 \<nuLinkL> N \<nuLinkR> x1) \<and> ([heap] p2 \<nuLinkL> M \<nuLinkR> x2)" unfolding Fusion_def Refining_ex by simp
+lemma [elim,\<nu>elim]: "(x1,x2) \<ratio> N1 \<nuFusion> N2 \<Longrightarrow> (x1 \<ratio> N1 \<Longrightarrow> x2 \<ratio> N2 \<Longrightarrow> C) \<Longrightarrow> C" unfolding Inhabited_def by auto
 
-lemma [\<nu>intro]: "\<nu>Share N s1 f1 \<Longrightarrow> \<nu>Share M s2 f2 \<Longrightarrow> \<nu>Share (N \<nuFusion> M) (s1 \<times>\<^sub>p s2) (\<lambda>z. map_prod (f1 z) (f2 z))" unfolding \<nu>Share_def by auto
-lemma [\<nu>intro]: "\<nu>CEqual N P eq1 \<Longrightarrow> \<nu>CEqual M Q eq2 \<Longrightarrow> \<nu>CEqual (N \<nuFusion> M) (P \<times>\<^sub>r Q) (eq1 \<times>\<^sub>r eq2)"unfolding \<nu>CEqual_def pair_forall by auto
-lemma [\<nu>intro]: "\<nu>Disposable \<tort_lbrace>x \<tycolon> X\<tort_rbrace> \<Longrightarrow> \<nu>Disposable \<tort_lbrace>y \<tycolon> Y\<tort_rbrace> \<Longrightarrow> \<nu>Disposable \<tort_lbrace>(x,y) \<tycolon> X \<nuFusion> Y\<tort_rbrace>" unfolding \<nu>Disposable_def pair_forall by auto
-lemma [\<nu>intro]: "\<nu>ShrIdentical N sid1 \<Longrightarrow> \<nu>ShrIdentical M sid2 \<Longrightarrow> \<nu>ShrIdentical (N \<nuFusion> M) (sid1 \<times>\<^sub>r sid2)" unfolding \<nu>ShrIdentical_def by (auto 0 4)
-lemma [\<nu>intro]: "\<nu>Ownership N ow1 \<Longrightarrow> \<nu>Ownership M ow2 \<Longrightarrow> \<nu>Ownership (N \<nuFusion> M) (ow1 \<times>\<^sub>o\<^sub>w ow2)" unfolding \<nu>Ownership_def by simp
 lemma [\<nu>intro]: "\<nu>Zero N z1 \<Longrightarrow> \<nu>Zero M z2 \<Longrightarrow> \<nu>Zero (N \<nuFusion> M) (z1,z2)" unfolding \<nu>Zero_def by simp
 
 lemma [\<nu>intro]: "\<^bold>c\<^bold>a\<^bold>s\<^bold>t x \<tycolon> N \<longmapsto> x' \<tycolon> N' \<^bold>m\<^bold>e\<^bold>a\<^bold>n\<^bold>w\<^bold>h\<^bold>i\<^bold>l\<^bold>e P \<Longrightarrow> \<^bold>c\<^bold>a\<^bold>s\<^bold>t y \<tycolon> M \<longmapsto> y' \<tycolon> M' \<^bold>m\<^bold>e\<^bold>a\<^bold>n\<^bold>w\<^bold>h\<^bold>i\<^bold>l\<^bold>e Q \<Longrightarrow>
@@ -565,10 +286,10 @@ subsection \<open>Lrep instantiations\<close>
 subsubsection \<open>lrep\<close>
 
 instantiation tuple :: (field_list) lrep begin
-definition llty_tuple :: " 'a tuple itself \<Rightarrow> llty " where [simp]: "llty_tuple _ = la_tup (llty TYPE('a))"
-definition disposable_tuple :: " 'a tuple \<Rightarrow> bool " where "disposable_tuple = pred_tuple disposable"
-lemma [simp]: "disposable (Tuple x) = disposable x" unfolding disposable_tuple_def by simp
-instance by standard
+definition llty_tuple :: " 'a tuple itself \<Rightarrow> llty " where [simp]: "llty_tuple _ = llty_tup (llty TYPE('a))"
+definition deepize_tuple :: " 'a tuple \<Rightarrow> deep_model " where "deepize_tuple x = DM_record (deepize (case_tuple id x))"
+definition shallowize_tuple :: " deep_model \<Rightarrow> 'a tuple " where "shallowize_tuple x = (case x of DM_record y \<Rightarrow> Tuple (shallowize y))"
+instance apply standard using shallowize_tuple_def deepize_tuple_def by (auto split: tuple.split)
 end
 
 subsubsection \<open>zero\<close>
@@ -578,65 +299,19 @@ definition zero_tuple :: " 'a tuple " where [simp]: "zero_tuple = Tuple 0"
 instance by standard
 end
 
-subsubsection \<open>shareable\<close>
-
-instantiation tuple :: ("{ownership,field_list}") ownership begin
-definition ownership_tuple :: " 'a tuple \<Rightarrow> ownership" where "ownership_tuple = case_tuple ownership"
-lemma [simp]: "ownership (Tuple a) = ownership a" unfolding ownership_tuple_def by simp
-instance by standard
-end
-
-instantiation tuple :: ("{sharing_identical,field_list}") sharing_identical begin
-definition sharing_identical_tuple :: " 'a tuple \<Rightarrow> 'a tuple \<Rightarrow> bool " where "sharing_identical_tuple = rel_tuple sharing_identical"
-lemma [simp]: "sharing_identical (Tuple a) (Tuple b) \<longleftrightarrow> sharing_identical a b" unfolding sharing_identical_tuple_def by simp
-instance proof
-  fix x y z :: " 'a tuple"  and a b :: zint
-  show "sharing_identical x x" by (cases x) simp
-  show "sharing_identical x y = sharing_identical y x" by (cases x, cases y) simp
-  show "sharing_identical x y \<Longrightarrow> sharing_identical y z \<Longrightarrow> sharing_identical x z" by (cases x, cases y, cases z) (auto intro: sharing_identical_trans)
-qed
-end
-
-instantiation tuple :: ("{share,field_list}") share begin
-definition shareable_tuple :: " 'a tuple \<Rightarrow> bool " where [simp]: "shareable_tuple = pred_tuple shareable"
-definition share_tuple :: " zint \<Rightarrow> 'a tuple \<Rightarrow> 'a tuple " where [simp]: "share_tuple z = map_tuple (share z)"
-definition dpriv_tuple :: " 'a tuple \<Rightarrow> 'a tuple " where "dpriv_tuple = map_tuple dpriv"
-lemma [simp]: "shareable (Tuple x) = shareable x" unfolding shareable_tuple_def by simp
-lemma [simp]: "share z (Tuple x) = Tuple (share z x)" unfolding share_tuple_def by simp
-lemma [simp]: "dpriv (Tuple a) = Tuple (dpriv a)" unfolding dpriv_tuple_def by simp
-instance proof
-  fix x y z :: " 'a tuple"  and a b :: zint
-  show "share (Gi 0) x = x" by (cases x) auto
-  show "share b (share a x) = share (a + b) x" by (cases x) auto
-qed
-end
-
 subsubsection \<open>ceq\<close>
 
 instantiation tuple :: ("{ceq,field_list}") ceq begin
-definition ceqable_tuple :: " 'a tuple \<Rightarrow> 'a tuple \<Rightarrow> bool " where "ceqable_tuple = rel_tuple ceqable"
+definition ceqable_tuple :: " heap \<Rightarrow> 'a tuple \<Rightarrow> 'a tuple \<Rightarrow> bool " where "ceqable_tuple heap = rel_tuple (ceqable heap)"
 definition ceq_tuple :: " 'a tuple \<Rightarrow> 'a tuple \<Rightarrow> bool " where "ceq_tuple = rel_tuple ceq"
-lemma [simp]: "ceqable (Tuple a) (Tuple b) = ceqable a b" unfolding ceqable_tuple_def by simp
+lemma [simp]: "ceqable heap (Tuple a) (Tuple b) = ceqable heap a b" unfolding ceqable_tuple_def by simp
 lemma [simp]: "ceq (Tuple a) (Tuple b) = ceq a b" unfolding ceq_tuple_def by simp
 instance proof
-  fix x y z :: " 'a tuple"
-  show "ceqable x y = ceqable y x" by (cases x; cases y) simp
-  show "ceqable x x \<Longrightarrow> ceq x x" by (cases x) auto
-  show "ceqable x y \<Longrightarrow> ceq x y = ceq y x" by (cases x; cases y) simp
-  show "ceqable x y \<Longrightarrow> ceqable y z \<Longrightarrow> ceqable x z \<Longrightarrow> ceq x y \<Longrightarrow> ceq y z \<Longrightarrow> ceq x z" by (cases x, cases y, cases z) (simp, blast intro: ceq_trans)
-qed
-end
-
-subsubsection \<open>naive\<close>
-
-instantiation tuple :: ("{naive_lrep,field_list}") naive_lrep begin
-instance proof
-  fix x y :: " 'a tuple " and z :: zint
-  show "disposable x = True" by (cases x) simp
-  show "shareable x = True" by (cases x) simp
-  show "dpriv x = x" by (cases x) simp
-  show " share z x = x" by (cases x) simp
-  show " sharing_identical x y = True" by (cases x; cases y) simp
+  fix x y z :: " 'a tuple" and h :: heap
+  show "ceqable h x y = ceqable h y x" by (cases x; cases y) simp
+  show "ceqable h x x \<Longrightarrow> ceq x x" by (cases x) auto
+  show "ceqable h x y \<Longrightarrow> ceq x y = ceq y x" by (cases x; cases y) simp
+  show "ceqable h x y \<Longrightarrow> ceqable h y z \<Longrightarrow> ceqable h x z \<Longrightarrow> ceq x y \<Longrightarrow> ceq y z \<Longrightarrow> ceq x z" by (cases x, cases y, cases z) (simp, blast intro: ceq_trans)
 qed
 end
 
@@ -647,184 +322,14 @@ instantiation tuple :: (field_list) field_list begin instance by standard end
 
 subsection \<open>Nu abstraction - `NuTuple`\<close>
 
-definition NuTuple :: "(('a::field_list), 'b) nu \<Rightarrow> ('a tuple, 'b) nu" ("\<lbrace> _ \<rbrace>") where "\<lbrace> N \<rbrace> p x = (case p of Tuple p' \<Rightarrow> p' \<nuLinkL> N \<nuLinkR> x)"
+definition NuTuple :: "(('a::field_list), 'b) \<nu> \<Rightarrow> ('a tuple, 'b) \<nu>" ("\<lbrace> _ \<rbrace>") where "\<lbrace> N \<rbrace> h p x = (case p of Tuple p' \<Rightarrow> [h] p' \<nuLinkL> N \<nuLinkR> x)"
 
-lemma [simp]: "Tuple p \<nuLinkL> \<lbrace> N \<rbrace> \<nuLinkR> x \<longleftrightarrow> p \<nuLinkL> N \<nuLinkR> x" unfolding NuTuple_def Refining_ex by simp
+lemma [simp]: "[heap] Tuple p \<nuLinkL> \<lbrace> N \<rbrace> \<nuLinkR> x \<longleftrightarrow> [heap] p \<nuLinkL> N \<nuLinkR> x" unfolding NuTuple_def Refining_ex by simp
 lemma [elim,\<nu>elim]: "x \<ratio> \<lbrace> N \<rbrace> \<Longrightarrow> (x \<ratio> N \<Longrightarrow> C) \<Longrightarrow> C" unfolding Inhabited_def tuple_exists by simp
 
-lemma [\<nu>intro]: "\<nu>Share N s f \<Longrightarrow> \<nu>Share \<lbrace> N \<rbrace> s f" unfolding \<nu>Share_def tuple_forall by simp
-lemma [\<nu>intro]: "\<nu>CEqual N P eq \<Longrightarrow> \<nu>CEqual \<lbrace> N \<rbrace> P eq" unfolding \<nu>CEqual_def tuple_forall by simp
-lemma [\<nu>intro]: "\<nu>Disposable \<tort_lbrace>x \<tycolon> X\<tort_rbrace> \<Longrightarrow> \<nu>Disposable \<tort_lbrace>x \<tycolon> \<lbrace> X \<rbrace>\<tort_rbrace>" unfolding \<nu>Disposable_def tuple_forall by simp
-lemma [\<nu>intro]: "\<nu>ShrIdentical N sid \<Longrightarrow> \<nu>ShrIdentical \<lbrace> N \<rbrace> sid" unfolding \<nu>ShrIdentical_def tuple_forall by simp
-lemma [\<nu>intro]: "\<nu>Ownership N ow \<Longrightarrow> \<nu>Ownership \<lbrace> N \<rbrace> ow" unfolding \<nu>Ownership_def tuple_forall by simp
+lemma [\<nu>intro]: "\<nu>Equal N P eq \<Longrightarrow> \<nu>Equal \<lbrace> N \<rbrace> P eq" unfolding \<nu>Equal_def tuple_forall by simp
 lemma [\<nu>intro]: "\<nu>Zero N z \<Longrightarrow> \<nu>Zero \<lbrace> N \<rbrace> z" unfolding \<nu>Zero_def by simp
-
-section \<open>Memory Witness\<close>
-
-datatype ('a::field) memcon = memcon \<open>(memadr, ('a::field)) map\<close>
-type_synonym 'a memobj = " 'a memcon owning"
-
-lemma memcon_forall[lrep_exps]: "All P \<longleftrightarrow> (\<forall>f. P (memcon f))" by (metis memcon.exhaust) 
-lemma memcon_exists[lrep_exps]: "Ex P \<longleftrightarrow> (\<exists>f. P (memcon f))" by (metis memcon.exhaust) 
-
-
-subsection \<open>Instantiations\<close>
-
-instantiation memcon :: (field) disposable begin
-definition disposable_memcon :: " 'a memcon \<Rightarrow> bool" where [simp]: "disposable_memcon _ = False"
-instance by standard
-end
-(*
-instantiation memcon :: ("{ownership, field}") ownership begin
-definition ownership_memcon :: " 'a memcon \<Rightarrow> ownership"
-  where "ownership_memcon x = (case x of memcon y \<Rightarrow> OWS_L (map ownership y))"
-lemma [simp]: "ownership (memcon p x) = OWS_L (map ownership x)"
-  unfolding ownership_memcon_def by simp
-instance by standard
-end *)
-
-instantiation memcon :: ( "{sharing_identical,ownership, field}") sharing_identical begin
-definition sharing_identical_memcon :: "  'a memcon \<Rightarrow> 'a memcon \<Rightarrow> bool"
-  where "sharing_identical_memcon = rel_memcon sharing_identical"
-
-lemma [simp]: "sharing_identical (memcon fa) (memcon fb) \<longleftrightarrow> (\<forall>x. rel_option sharing_identical (fa x) (fb x))"
-  unfolding sharing_identical_memcon_def by (auto simp add: rel_fun_def)
-instance proof
-  fix x y z :: " 'a memcon"
-  show "sharing_identical x x" apply (cases x) apply (simp add: lrep_exps)
-    by (simp add: list_all2_refl option.rel_refl) 
-  show "sharing_identical x y = sharing_identical y x"
-    apply (cases x; cases y; simp; rule)
-    subgoal premises prems for xa xaa apply rule subgoal for x
-      by (insert prems(3)[THEN spec, of x]; cases \<open>xaa x\<close>; cases \<open>xa x\<close>) (auto simp add: list_all2_conv_all_nth)
-    done
-    subgoal premises prems for xa xaa apply rule subgoal for x
-      by (insert prems(3)[THEN spec, of x]; cases \<open>xaa x\<close>; cases \<open>xa x\<close>) (auto simp add: list_all2_conv_all_nth)
-    done done
-  show "sharing_identical x y \<Longrightarrow> sharing_identical y z \<Longrightarrow> sharing_identical x z"
-    apply (cases x; cases y; cases z; simp) subgoal premises prems for xa xaa xb apply rule subgoal for x 
-        apply (insert prems(1)[THEN spec, of x] prems(2)[THEN spec, of x]; cases "xa x"; cases "xb x"; cases "xaa x")
-        apply (auto simp add: list_all2_conv_all_nth)
-        by (meson sharing_identical_sym sharing_identical_trans)
-      done done
-qed
-end
-
-subsection \<open>Image: object\<close>
-
-datatype 'a object = object memadr 'a (infixr "\<R_arr_tail>" 60)
-
-abbreviation "adr_of_object obj \<equiv> (case obj of a \<R_arr_tail> x \<Rightarrow> a)"
-abbreviation "x_of_object obj \<equiv> (case obj of a \<R_arr_tail> x \<Rightarrow> x)"
-
-lemma object_forall[lrep_exps]: "All P \<longleftrightarrow> (\<forall>a x. P (a \<R_arr_tail> x))" by (metis object.exhaust)
-lemma object_exists[lrep_exps]: "Ex P \<longleftrightarrow> (\<exists>a x. P (a \<R_arr_tail> x))" by (metis object.exhaust)
-
-subsection \<open>\<nu>-abstraction : MemMap\<close>
-
-definition MemMap :: "(('a::field), 'b) nu \<Rightarrow> ('a memobj, (memadr, 'b) map owning) nu"
-  where "MemMap N p x = (
-    case (p,x) of (zp \<left_fish_tail> memcon f, z \<left_fish_tail> g) \<Rightarrow>
-        (zp = z) \<and> (\<forall>adr. rel_option (\<lambda>p x. p \<nuLinkL> N \<nuLinkR> x) (f adr) (g adr))
-    | (\<down_fish_tail> , \<down_fish_tail>) \<Rightarrow> True | _ \<Rightarrow> False)"
-
-lemma [simp]: "zp \<left_fish_tail> memcon f \<nuLinkL> MemMap N \<nuLinkR> z \<left_fish_tail> g \<longleftrightarrow>
-    (zp = z) \<and> (\<forall>adr. rel_option (\<lambda>p x. p \<nuLinkL> N \<nuLinkR> x) (f adr) (g adr))"
-  and [simp]: "\<down_fish_tail> \<nuLinkL> MemMap N \<nuLinkR> x' \<longleftrightarrow> x' = \<down_fish_tail>" and [simp]: "p' \<nuLinkL> MemMap N \<nuLinkR> \<down_fish_tail> \<longleftrightarrow> p' = \<down_fish_tail>"
-  unfolding MemMap_def Refining_ex by (auto simp add: memptr_forall split: memcon.split owning.split)
-
-lemma [elim,\<nu>elim]: "z \<left_fish_tail> f \<ratio> MemMap N \<Longrightarrow> ((\<And>x. f adr = Some x \<Longrightarrow> x \<ratio> N) \<Longrightarrow> C) \<Longrightarrow> C"
-  unfolding Inhabited_def apply (auto 6 6 simp add: lrep_exps list_all2_conv_all_nth)
-  by (metis memadr.exhaust option_rel_Some2)  
-
-lemma [\<nu>intro]: "\<nu>Share (MemMap N) (\<lambda>x. True) share"
-  unfolding \<nu>Share_def by (simp add: owning_forall memcon_forall memptr_forall object_forall)
-lemma [\<nu>intro]: "\<nu>Disposable \<tort_lbrace>\<down_fish_tail> \<tycolon> MemMap N\<tort_rbrace>" unfolding \<nu>Disposable_def by simp
-lemma [\<nu>intro]: "\<nu>CEqual (MemMap N) (\<lambda>x y. True) (\<lambda>x y. True)" unfolding \<nu>CEqual_def by simp
-lemma [\<nu>intro]: "\<nu>Ownership (MemMap N) ownership"
-  unfolding \<nu>Ownership_def by (simp add: owning_forall memcon_forall memptr_forall object_exists)
-lemma [\<nu>intro]: "\<nu>Zero (MemMap N) \<down_fish_tail>" unfolding \<nu>Zero_def by simp
-
-section \<open>Ghost\<close>
-
-datatype 'a ghost = ghost 'a
-
-lemma ghost_forall[lrep_exps]: "All P \<longleftrightarrow> (\<forall>x. P (ghost x))" by (metis ghost.exhaust)
-lemma ghost_exists[lrep_exps]: "Ex P \<longleftrightarrow> (\<exists>x. P (ghost x))" by (metis ghost.exhaust)
-
-subsection \<open>Instantiations\<close>
-
-instantiation ghost :: (type) field begin
-definition llty_ghost :: " 'a ghost itself \<Rightarrow> llty" where [simp]: "llty_ghost _ = la_z"
-definition disposable_ghost :: " 'a ghost \<Rightarrow> bool " where [simp]: "disposable_ghost _ = True"
-instance by standard
-end
-
-lemma [\<nu>intro]: "\<nu>Disposable S" for S :: " 'a ghost set " unfolding \<nu>Disposable_def by simp
-
-instantiation ghost :: (type) field_list begin instance by standard end
-
-instantiation ghost :: (type) ceq begin
-definition ceqable_ghost :: " 'a ghost \<Rightarrow> 'a ghost \<Rightarrow> bool" where [simp]: "ceqable_ghost _ _ = True"
-definition ceq_ghost :: " 'a ghost \<Rightarrow> 'a ghost \<Rightarrow> bool" where [simp]: "ceq_ghost _ _ = True"
-instance by standard auto
-end
-
-instantiation ghost :: (type) sharing_identical begin
-definition sharing_identical_ghost :: "'a ghost \<Rightarrow> 'a ghost \<Rightarrow> bool" where [simp]: "sharing_identical_ghost _ _ = True"
-instance by standard auto
-end
-
-instantiation ghost :: (type) share begin
-definition shareable_ghost :: "'a ghost \<Rightarrow> bool" where [simp]: "shareable_ghost _ = True"
-definition share_ghost :: "zint \<Rightarrow> 'a ghost \<Rightarrow> 'a ghost" where [simp]: "share_ghost _ x = x"
-definition dpriv_ghost :: "'a ghost \<Rightarrow> 'a ghost" where [simp]: "dpriv_ghost x = x"
-instance by standard auto
-end
-
-instantiation ghost :: (type) ownership begin
-definition ownership_ghost :: " 'a ghost \<Rightarrow> ownership" where [simp]: "ownership_ghost _ = OWS_0"
-instance by standard
-end
-
-lemma [\<nu>intro]: "\<nu>Ownership N (\<lambda>_. OWS_0)" for N :: "('a ghost, 'b) nu" unfolding \<nu>Ownership_def by simp
-
-instantiation ghost :: (zero) zero begin
-definition zero_ghost :: " 'a ghost" where [simp]: "zero_ghost = ghost 0"
-instance by standard
-end
-
-subsubsection \<open>\<nu>-abstraction\<close>
-
-definition Ghost :: "('a ghost, 'a) nu" where "Ghost p x \<longleftrightarrow> (case p of ghost p' \<Rightarrow> p' = x)"
-
-lemma [simp]: "ghost p \<nuLinkL> Ghost \<nuLinkR> x \<longleftrightarrow> p = x" unfolding Ghost_def Refining_ex by auto
-
-lemma [\<nu>intro]: "\<nu>Share Ghost (\<lambda>x. True) (\<lambda>z x. x)" unfolding \<nu>Share_def by simp
-lemma [\<nu>intro]: "\<nu>ShrIdentical Ghost (\<lambda>_ _. True)" unfolding \<nu>ShrIdentical_def by simp
-lemma [\<nu>intro]: "\<nu>CEqual Ghost (\<lambda>_ _. True) (\<lambda>_ _. True)" unfolding \<nu>CEqual_def by simp
-lemma [\<nu>intro]: "\<nu>Deprive Ghost (\<lambda>x. x)" unfolding \<nu>Deprive_def by simp
-lemma [\<nu>intro]: "\<nu>Zero Ghost 0" unfolding \<nu>Zero_def by simp
-
-(* definition MemObj :: "(('a::field), 'b) nu \<Rightarrow> ('a memobj, 'b object owning) nu"
-  where "MemObj N p x = (
-    case (p,x) of (zp \<left_fish_tail> memcon adrp p , z \<left_fish_tail> (adrx \<R_arr_tail> x)) \<Rightarrow> (zp = z) \<and> (adrp = adrx) \<and> (p \<nuLinkL> N \<nuLinkR> x)
-        | (\<down_fish_tail> , \<down_fish_tail>) \<Rightarrow> True | _ \<Rightarrow> False)"
-
-lemma [simp]: "zp \<left_fish_tail> memcon adrp p \<nuLinkL> MemObj N \<nuLinkR> z \<left_fish_tail> adrx \<R_arr_tail> x \<longleftrightarrow> (zp = z) \<and> (adrp = adrx) \<and> (p \<nuLinkL> N \<nuLinkR> x)"
-  and [simp]: "\<down_fish_tail> \<nuLinkL> MemObj N \<nuLinkR> x' \<longleftrightarrow> x' = \<down_fish_tail>" and [simp]: "p' \<nuLinkL> MemObj N \<nuLinkR> \<down_fish_tail> \<longleftrightarrow> p' = \<down_fish_tail>"
-  unfolding MemObj_def Refining_ex by  (auto simp add: memptr_forall split: memcon.split owning.split)
-
-lemma [\<nu>intro]: "\<nu>Share (MemObj N) (\<lambda>x. True) share"
-  unfolding \<nu>Share_def by (simp add: owning_forall memcon_forall memptr_forall object_forall)
-lemma [\<nu>intro]: "\<nu>Disposable \<tort_lbrace>\<down_fish_tail> \<tycolon> MemObj N\<tort_rbrace>" unfolding \<nu>Disposable_def by simp
-lemma [\<nu>intro]: "\<nu>CEqual (MemObj N) (\<lambda>x y. True) (\<lambda>x y. True)" unfolding \<nu>CEqual_def by simp
-lemma [\<nu>intro]: "\<nu>Ownership (MemObj N) ownership"
-  unfolding \<nu>Ownership_def by (simp add: owning_forall memcon_forall memptr_forall object_exists)
-lemma [\<nu>intro]: "\<nu>Ownership N ow \<Longrightarrow> \<nu>ShrIdentical (MemObj N) (rel_owning (rel_object (inv_imagep (=) ow)))"
-  unfolding \<nu>Ownership_def \<nu>ShrIdentical_def
-  by (simp add: owning_forall memcon_forall memptr_forall object_exists owning_exists) auto
-lemma [\<nu>intro]: "\<nu>Zero (MemObj N) \<down_fish_tail>" unfolding \<nu>Zero_def by simp
-*)
+lemma [\<nu>intro]: "NuSet \<tort_lbrace> x \<tycolon> T \<tort_rbrace> \<Longrightarrow> NuSet \<tort_lbrace> x \<tycolon> \<lbrace> T \<rbrace> \<tort_rbrace>" unfolding NuSet_def by (simp add: lrep_exps)
+lemma [\<nu>intro]: "\<nu>Resources T rcss \<Longrightarrow> \<nu>Resources \<lbrace> T \<rbrace> rcss" unfolding \<nu>def by (simp add: lrep_exps)
 
 end
